<?xml version="1.0"?>
<rdf:RDF xmlns="http://www.estrellaproject.org/lkif-core/time.owl#"
     xml:base="http://www.estrellaproject.org/lkif-core/time.owl"
     xmlns:owl="http://www.w3.org/2002/07/owl#"
     xmlns:rdf="http://www.w3.org/1999/02/22-rdf-syntax-ns#"
     xmlns:xml="http://www.w3.org/XML/1998/namespace"
     xmlns:xsd="http://www.w3.org/2001/XMLSchema#"
     xmlns:daml="http://www.daml.org/2001/03/daml+oil#"
     xmlns:owl2="http://www.w3.org/2006/12/owl2#"
     xmlns:rdfs="http://www.w3.org/2000/01/rdf-schema#"
     xmlns:time="http://www.estrellaproject.org/lkif-core/time.owl#"
     xmlns:mereo="http://www.estrellaproject.org/lkif-core/mereology.owl#"
     xmlns:opla-sd="http://ontologydesignpatterns.org/opla-sd#"
     xmlns:owl2xml="http://www.w3.org/2006/12/owl2-xml#"
     xmlns:lkif-top="http://www.estrellaproject.org/lkif-core/lkif-top.owl#">
    <owl:Ontology rdf:about="http://www.estrellaproject.org/lkif-core/time.owl">
        <owl:imports rdf:resource="http://www.estrellaproject.org/lkif-core/mereology.owl"/>
        <rdfs:comment>An ontology of time based on &quot;Actions and Events in Interval Logc&quot; by James F. Allen and George Ferguson, 1994.  This ontology is similar to the W3C best practices OWL-Time ontology draft of 18 May 2006 by Jerry R. Hobbs and Feng Pan (http://www.w3.org/2001/sw/BestPractices/OEP/Time-Ontology).  Meta-physical time concepts are separated from parts dealing with quantitative time.  Relations were strengthened with more axioms.</rdfs:comment>
        <owl:versionInfo>LKIF Core, version 1.1, copyright (C) 2008, the ESTRELLA consortium</owl:versionInfo>
        <owl:versionInfo>Partner contributions from the University of Amsterdam (UvA) and the University of Bologna (UNIBO).

Editor:       Rinke Hoekstra (UvA)
Authors:      Rinke Hoekstra (UvA), Alexander Boer (UvA), Kasper van den Berg (UvA)
Contributors: Joost Breuker (UvA), Monica Palmirani (UNIBO)</owl:versionInfo>
        <owl:versionInfo>The LKIF-Core ontology, version 1.0, is part of Deliverable 1.4 of the European project for Standardised Transparent Representations in order to Extend Legal Accessibility (ESTRELLA, IST-2004-027665), http://www.estrellaproject.org

The use of this ontology, and the OWL files through which it is distributed, is covered by the GNU Lesser General Public License (LGPL), version 2.1 (http://www.gnu.org/copyleft/lesser.html) in as far as the copyright is not covered by additional restrictions of the ESTRELLA consortium agreement (info@estrellaproject.org). The LGPL license places copyright restrictions on the ontology itself but does not apply these restrictions to software that merely links with concepts defined in the ontology library. Please read the license restrictions before using this work.</owl:versionInfo>
        <owl:versionInfo>This module is part of LKIF-Core, version 1.1, part of Deliverable 1.4 of ESTRELLA, IST-2004-027665</owl:versionInfo>
    </owl:Ontology>
    


    <!-- 
    ///////////////////////////////////////////////////////////////////////////////////////
    //
    // Object Properties
    //
    ///////////////////////////////////////////////////////////////////////////////////////
     -->

    


    <!-- http://www.estrellaproject.org/lkif-core/mereology.owl#component -->

    <owl:ObjectProperty rdf:about="http://www.estrellaproject.org/lkif-core/mereology.owl#component"/>
    


    <!-- http://www.estrellaproject.org/lkif-core/time.owl#after -->

    <owl:ObjectProperty rdf:about="http://www.estrellaproject.org/lkif-core/time.owl#after">
        <rdfs:subPropertyOf rdf:resource="http://www.estrellaproject.org/lkif-core/time.owl#temporal_relation"/>
        <owl:inverseOf rdf:resource="http://www.estrellaproject.org/lkif-core/time.owl#before"/>
        <rdf:type rdf:resource="http://www.w3.org/2002/07/owl#TransitiveProperty"/>
        <rdfs:domain rdf:resource="http://www.estrellaproject.org/lkif-core/time.owl#Temporal_Occurrence"/>
        <rdfs:range rdf:resource="http://www.estrellaproject.org/lkif-core/time.owl#Temporal_Occurrence"/>
        <rdfs:comment>&apos;after&apos; is the transitive closure of &apos;next&apos;; this is defined in time-rules.owl.</rdfs:comment>
        <rdfs:comment>Specifies that a time period occurs after another period, but might overlap with it.</rdfs:comment>
    </owl:ObjectProperty>
    


    <!-- http://www.estrellaproject.org/lkif-core/time.owl#before -->

    <owl:ObjectProperty rdf:about="http://www.estrellaproject.org/lkif-core/time.owl#before">
        <rdfs:subPropertyOf rdf:resource="http://www.estrellaproject.org/lkif-core/time.owl#temporal_relation"/>
        <rdf:type rdf:resource="http://www.w3.org/2002/07/owl#TransitiveProperty"/>
        <rdfs:domain rdf:resource="http://www.estrellaproject.org/lkif-core/time.owl#Temporal_Occurrence"/>
        <rdfs:range rdf:resource="http://www.estrellaproject.org/lkif-core/time.owl#Temporal_Occurrence"/>
        <rdfs:comment>Specifies that a time period occurs before another period, but might overlap with it.</rdfs:comment>
    </owl:ObjectProperty>
    


    <!-- http://www.estrellaproject.org/lkif-core/time.owl#between -->

    <owl:ObjectProperty rdf:about="http://www.estrellaproject.org/lkif-core/time.owl#between">
        <rdfs:subPropertyOf rdf:resource="http://www.estrellaproject.org/lkif-core/time.owl#temporal_relation"/>
        <rdfs:domain rdf:resource="http://www.estrellaproject.org/lkif-core/time.owl#Temporal_Occurrence"/>
        <rdfs:range rdf:resource="http://www.estrellaproject.org/lkif-core/time.owl#Pair_Of_Periods"/>
        <rdfs:comment>Specifies that a time period occurs between two other periods</rdfs:comment>
    </owl:ObjectProperty>
    


    <!-- http://www.estrellaproject.org/lkif-core/time.owl#during -->

    <owl:ObjectProperty rdf:about="http://www.estrellaproject.org/lkif-core/time.owl#during">
        <rdfs:subPropertyOf rdf:resource="http://www.estrellaproject.org/lkif-core/time.owl#temporal_relation"/>
        <rdfs:comment>Specifies that a time period occurs during another period</rdfs:comment>
    </owl:ObjectProperty>
    


    <!-- http://www.estrellaproject.org/lkif-core/time.owl#finishes -->

    <owl:ObjectProperty rdf:about="http://www.estrellaproject.org/lkif-core/time.owl#finishes">
        <rdfs:subPropertyOf rdf:resource="http://www.estrellaproject.org/lkif-core/time.owl#temporal_relation"/>
        <rdfs:comment>Specifies that a time period finishes another period, i.e. the other period starts before, but ends at the same moment</rdfs:comment>
    </owl:ObjectProperty>
    


    <!-- http://www.estrellaproject.org/lkif-core/time.owl#immediately_after -->

    <owl:ObjectProperty rdf:about="http://www.estrellaproject.org/lkif-core/time.owl#immediately_after">
        <rdfs:subPropertyOf rdf:resource="http://www.estrellaproject.org/lkif-core/time.owl#after"/>
        <owl:inverseOf rdf:resource="http://www.estrellaproject.org/lkif-core/time.owl#immediately_before"/>
        <rdfs:domain rdf:resource="http://www.estrellaproject.org/lkif-core/time.owl#Temporal_Occurrence"/>
        <rdfs:range rdf:resource="http://www.estrellaproject.org/lkif-core/time.owl#Temporal_Occurrence"/>
        <rdfs:comment>&apos;is_met_by&apos; is renamed to &apos;immediately_after&apos;</rdfs:comment>
        <rdfs:comment>Add to OWL 1.1: &apos;immediately_after&apos; is serial, &apos;immediately_after&apos; is irreflexive</rdfs:comment>
        <rdfs:comment>Specifies that a time period occurs immediately after another period, i.e. it starts where the other period ends</rdfs:comment>
    </owl:ObjectProperty>
    


    <!-- http://www.estrellaproject.org/lkif-core/time.owl#immediately_before -->

    <owl:ObjectProperty rdf:about="http://www.estrellaproject.org/lkif-core/time.owl#immediately_before">
        <rdfs:subPropertyOf rdf:resource="http://www.estrellaproject.org/lkif-core/time.owl#before"/>
        <rdfs:domain rdf:resource="http://www.estrellaproject.org/lkif-core/time.owl#Temporal_Occurrence"/>
        <rdfs:range rdf:resource="http://www.estrellaproject.org/lkif-core/time.owl#Temporal_Occurrence"/>
        <rdfs:comment>&apos;meet&apos; in Allen&apos;s paper is replaced by &apos;immediately_before&apos;</rdfs:comment>
        <rdfs:comment>Add to OWL 1.1: &apos;immediately_before&apos; is serial, &apos;immediately_before&apos; is irreflexive</rdfs:comment>
        <rdfs:comment>Specifies that a time period occurs immediately before another period, i.e. it ends where the other period starts</rdfs:comment>
        <rdfs:comment>t1 previous t2: interval t1 is before t2, but there is no interval between them, i.e., t1 ends where t2 starts</rdfs:comment>
    </owl:ObjectProperty>
    


    <!-- http://www.estrellaproject.org/lkif-core/time.owl#overlap -->

    <owl:ObjectProperty rdf:about="http://www.estrellaproject.org/lkif-core/time.owl#overlap">
        <rdfs:subPropertyOf rdf:resource="http://www.estrellaproject.org/lkif-core/time.owl#temporal_relation"/>
        <rdfs:comment>Specifies that a time period overlaps with another time period (in any way)</rdfs:comment>
    </owl:ObjectProperty>
    


    <!-- http://www.estrellaproject.org/lkif-core/time.owl#preceeds -->

    <owl:ObjectProperty rdf:about="http://www.estrellaproject.org/lkif-core/time.owl#preceeds">
        <rdfs:subPropertyOf rdf:resource="http://www.estrellaproject.org/lkif-core/time.owl#temporal_relation"/>
        <rdfs:comment>Specifies that a time period preceeds another period, the periods do not overlap</rdfs:comment>
    </owl:ObjectProperty>
    


    <!-- http://www.estrellaproject.org/lkif-core/time.owl#starts -->

    <owl:ObjectProperty rdf:about="http://www.estrellaproject.org/lkif-core/time.owl#starts">
        <rdfs:subPropertyOf rdf:resource="http://www.estrellaproject.org/lkif-core/time.owl#temporal_relation"/>
        <rdfs:comment>Specifies that a time period starts another period, i.e. the other period starts at the same time, but ends at a later time.</rdfs:comment>
    </owl:ObjectProperty>
    


    <!-- http://www.estrellaproject.org/lkif-core/time.owl#temporal_relation -->

    <owl:ObjectProperty rdf:about="http://www.estrellaproject.org/lkif-core/time.owl#temporal_relation">
        <rdfs:domain rdf:resource="http://www.estrellaproject.org/lkif-core/time.owl#Temporal_Occurrence"/>
        <rdfs:range rdf:resource="http://www.estrellaproject.org/lkif-core/time.owl#Temporal_Occurrence"/>
        <rdfs:comment>A relation between two time periods</rdfs:comment>
    </owl:ObjectProperty>
    


    <!-- 
    ///////////////////////////////////////////////////////////////////////////////////////
    //
    // Classes
    //
    ///////////////////////////////////////////////////////////////////////////////////////
     -->

    


    <!-- http://www.estrellaproject.org/lkif-core/lkif-top.owl#Spatio_Temporal_Occurrence -->

    <owl:Class rdf:about="http://www.estrellaproject.org/lkif-core/lkif-top.owl#Spatio_Temporal_Occurrence">
        <opla-sd:entityPosition>
            <rdf:Description>
                <opla-sd:entityPositionX rdf:datatype="http://www.w3.org/2001/XMLSchema#double">69.15778384019748</opla-sd:entityPositionX>
                <opla-sd:entityPositionY rdf:datatype="http://www.w3.org/2001/XMLSchema#double">72.33271120637436</opla-sd:entityPositionY>
                <rdfs:comment xml:lang="en">This is an entity positioning annotation generated by CoModIDE (https://comodide.com/). Removing this annotation will break rendering the CoModIDE schema diagram view.</rdfs:comment>
            </rdf:Description>
        </opla-sd:entityPosition>
    </owl:Class>
    


    <!-- http://www.estrellaproject.org/lkif-core/mereology.owl#Atom -->

    <owl:Class rdf:about="http://www.estrellaproject.org/lkif-core/mereology.owl#Atom">
        <opla-sd:entityPosition>
            <rdf:Description>
                <opla-sd:entityPositionX rdf:datatype="http://www.w3.org/2001/XMLSchema#double">100.2977078301256</opla-sd:entityPositionX>
                <opla-sd:entityPositionY rdf:datatype="http://www.w3.org/2001/XMLSchema#double">460.1366976561822</opla-sd:entityPositionY>
                <rdfs:comment xml:lang="en">This is an entity positioning annotation generated by CoModIDE (https://comodide.com/). Removing this annotation will break rendering the CoModIDE schema diagram view.</rdfs:comment>
            </rdf:Description>
        </opla-sd:entityPosition>
    </owl:Class>
    


    <!-- http://www.estrellaproject.org/lkif-core/mereology.owl#Composition -->

    <owl:Class rdf:about="http://www.estrellaproject.org/lkif-core/mereology.owl#Composition">
        <opla-sd:entityPosition>
            <rdf:Description>
                <opla-sd:entityPositionX rdf:datatype="http://www.w3.org/2001/XMLSchema#double">40.30174900383285</opla-sd:entityPositionX>
                <opla-sd:entityPositionY rdf:datatype="http://www.w3.org/2001/XMLSchema#double">330.2679238827894</opla-sd:entityPositionY>
                <rdfs:comment xml:lang="en">This is an entity positioning annotation generated by CoModIDE (https://comodide.com/). Removing this annotation will break rendering the CoModIDE schema diagram view.</rdfs:comment>
            </rdf:Description>
        </opla-sd:entityPosition>
    </owl:Class>
    


    <!-- http://www.estrellaproject.org/lkif-core/mereology.owl#Pair -->

    <owl:Class rdf:about="http://www.estrellaproject.org/lkif-core/mereology.owl#Pair">
        <opla-sd:entityPosition>
            <rdf:Description>
                <opla-sd:entityPositionX rdf:datatype="http://www.w3.org/2001/XMLSchema#double">439.6949379796432</opla-sd:entityPositionX>
                <opla-sd:entityPositionY rdf:datatype="http://www.w3.org/2001/XMLSchema#double">489.6338477964495</opla-sd:entityPositionY>
                <rdfs:comment xml:lang="en">This is an entity positioning annotation generated by CoModIDE (https://comodide.com/). Removing this annotation will break rendering the CoModIDE schema diagram view.</rdfs:comment>
            </rdf:Description>
        </opla-sd:entityPosition>
    </owl:Class>
    


    <!-- http://www.estrellaproject.org/lkif-core/time.owl#Interval -->

    <owl:Class rdf:about="http://www.estrellaproject.org/lkif-core/time.owl#Interval">
        <rdfs:subClassOf rdf:resource="http://www.estrellaproject.org/lkif-core/mereology.owl#Composition"/>
        <rdfs:subClassOf rdf:resource="http://www.estrellaproject.org/lkif-core/time.owl#Temporal_Occurrence"/>
        <owl:disjointWith rdf:resource="http://www.estrellaproject.org/lkif-core/time.owl#Moment"/>
        <opla-sd:entityPosition>
            <rdf:Description>
                <opla-sd:entityPositionX rdf:datatype="http://www.w3.org/2001/XMLSchema#double">210.36151085061408</opla-sd:entityPositionX>
                <opla-sd:entityPositionY rdf:datatype="http://www.w3.org/2001/XMLSchema#double">229.90072435404153</opla-sd:entityPositionY>
                <rdfs:comment xml:lang="en">This is an entity positioning annotation generated by CoModIDE (https://comodide.com/). Removing this annotation will break rendering the CoModIDE schema diagram view.</rdfs:comment>
            </rdf:Description>
        </opla-sd:entityPosition>
        <rdfs:comment>An interval is a composition of multiple periods of time.</rdfs:comment>
    </owl:Class>
    


    <!-- http://www.estrellaproject.org/lkif-core/time.owl#Moment -->

    <owl:Class rdf:about="http://www.estrellaproject.org/lkif-core/time.owl#Moment">
        <rdfs:subClassOf rdf:resource="http://www.estrellaproject.org/lkif-core/mereology.owl#Atom"/>
        <rdfs:subClassOf rdf:resource="http://www.estrellaproject.org/lkif-core/time.owl#Temporal_Occurrence"/>
        <opla-sd:entityPosition>
            <rdf:Description>
                <opla-sd:entityPositionX rdf:datatype="http://www.w3.org/2001/XMLSchema#double">389.6223853828925</opla-sd:entityPositionX>
                <opla-sd:entityPositionY rdf:datatype="http://www.w3.org/2001/XMLSchema#double">289.5160734777976</opla-sd:entityPositionY>
                <rdfs:comment xml:lang="en">This is an entity positioning annotation generated by CoModIDE (https://comodide.com/). Removing this annotation will break rendering the CoModIDE schema diagram view.</rdfs:comment>
            </rdf:Description>
        </opla-sd:entityPosition>
        <rdfs:comment>A moment is an atomic period of time, i.e. it cannot be divided into other parts</rdfs:comment>
    </owl:Class>
    


    <!-- http://www.estrellaproject.org/lkif-core/time.owl#Pair_Of_Periods -->

    <owl:Class rdf:about="http://www.estrellaproject.org/lkif-core/time.owl#Pair_Of_Periods">
        <rdfs:subClassOf rdf:resource="http://www.estrellaproject.org/lkif-core/mereology.owl#Pair"/>
        <rdfs:subClassOf>
            <owl:Restriction>
                <owl:onProperty rdf:resource="http://www.estrellaproject.org/lkif-core/mereology.owl#component"/>
                <owl:allValuesFrom rdf:resource="http://www.estrellaproject.org/lkif-core/time.owl#Temporal_Occurrence"/>
            </owl:Restriction>
        </rdfs:subClassOf>
        <opla-sd:entityPosition>
            <rdf:Description>
                <opla-sd:entityPositionX rdf:datatype="http://www.w3.org/2001/XMLSchema#double">519.9521868240665</opla-sd:entityPositionX>
                <opla-sd:entityPositionY rdf:datatype="http://www.w3.org/2001/XMLSchema#double">399.88817109743707</opla-sd:entityPositionY>
                <rdfs:comment xml:lang="en">This is an entity positioning annotation generated by CoModIDE (https://comodide.com/). Removing this annotation will break rendering the CoModIDE schema diagram view.</rdfs:comment>
            </rdf:Description>
        </opla-sd:entityPosition>
        <rdfs:comment>A pair of two time periods</rdfs:comment>
    </owl:Class>
    


    <!-- http://www.estrellaproject.org/lkif-core/time.owl#Temporal_Occurrence -->

    <owl:Class rdf:about="http://www.estrellaproject.org/lkif-core/time.owl#Temporal_Occurrence">
        <rdfs:subClassOf rdf:resource="http://www.estrellaproject.org/lkif-core/lkif-top.owl#Spatio_Temporal_Occurrence"/>
        <rdfs:subClassOf>
            <owl:Class>
                <owl:intersectionOf rdf:parseType="Collection">
                    <owl:Restriction>
                        <owl:onProperty rdf:resource="http://www.estrellaproject.org/lkif-core/time.owl#immediately_after"/>
                        <owl:someValuesFrom rdf:resource="http://www.estrellaproject.org/lkif-core/time.owl#Temporal_Occurrence"/>
                    </owl:Restriction>
                    <owl:Restriction>
                        <owl:onProperty rdf:resource="http://www.estrellaproject.org/lkif-core/time.owl#immediately_before"/>
                        <owl:someValuesFrom rdf:resource="http://www.estrellaproject.org/lkif-core/time.owl#Temporal_Occurrence"/>
                    </owl:Restriction>
                </owl:intersectionOf>
            </owl:Class>
        </rdfs:subClassOf>
        <opla-sd:entityPosition>
            <rdf:Description>
                <opla-sd:entityPositionX rdf:datatype="http://www.w3.org/2001/XMLSchema#double">560.2277242342268</opla-sd:entityPositionX>
                <opla-sd:entityPositionY rdf:datatype="http://www.w3.org/2001/XMLSchema#double">69.68874859065323</opla-sd:entityPositionY>
                <rdfs:comment xml:lang="en">This is an entity positioning annotation generated by CoModIDE (https://comodide.com/). Removing this annotation will break rendering the CoModIDE schema diagram view.</rdfs:comment>
            </rdf:Description>
        </opla-sd:entityPosition>
        <rdfs:comment>A period of time, has a duration</rdfs:comment>
    </owl:Class>
</rdf:RDF>



<!-- Generated by the OWL API (version 4.5.29.2024-05-13T12:11:03Z) https://github.com/owlcs/owlapi -->

